\documentclass[french,10pt]{article}
\input preambule_2013

\newcommand\Resultat[1]{%
\multicolumn{3}{l}{\pfr{#1}}%
}

\begin{document}

\begin{center}
	\textbf{\bsc{Sujet A}}
\end{center}

\textbf{Développements :}
\[
\begin{array}[t]{rcl}
	A(x) & = & 3(2x - 4) \\
	A(x) & = & 3 \times 2x - 3 \times 4 \\
	\Resultat{A(x) = 6x - 12}
\end{array}
\qq
\begin{array}[t]{rcl}
	B(x) & = & (6x + 2)(-2x - 3) \\
	B(x) & = & -12x^2 - 18x - 4x - 6 \\
	\Resultat{B(x) = -12x^2 - 24x - 6}
\end{array}
\qq
\begin{array}[t]{rcl}
	C(x) & = & (5 - 2x)^2 \\
	C(x) & = & 5^2 - 2 \times 5 \times 2x + (2x)^2\\
	\Resultat{C(x) = 4x^2 - 20x + 25}
\end{array}
\]

\textbf{Factorisations :}
\[
\begin{array}[t]{rcl}
	D(x) & = & 4x + 8 \\
	D(x) & = & 4x + 4 \times 2 \\
	\Resultat{D(x) = 4(x + 2)}
\end{array}
\qq
\begin{array}[t]{rcl}
	E(x) & = & (3x + 1)(-2x - 1) + (3x + 1)(x + 3) \\
	E(x) & = & (3x + 1)[(-2x - 1) + (x + 3)] \\
	E(x) & = & (3x + 1)(-2x - 1 + x + 3) \\
	\Resultat{E(x) = (3x + 1)(-x + 2)}
\end{array}
\qq
\begin{array}[t]{rcl}
	F(x) & = & (x - 4)^2 - (2x + 3)^2 \\
	F(x) & = & [(x - 4) + (2x + 3)] \times [(x - 4) - (2x + 3)] \\
	F(x) & = & (x - 4 + 2x + 3)(x - 4 - 2x - 3) \\
	\Resultat{F(x) = (3x - 1)(-x - 7)}
\end{array}
\]

\textbf{\'Equations :}
\[\begin{array}[t]{crcl}
	& 4x - 3 & = & 7 \\
	\Leftrightarrow & 4x - 3 + 3 & = & 7 + 3 \\
	\Leftrightarrow & 4x & = & 10 \\
	\Leftrightarrow & x & = & \frac{10}{4} \\
	\Leftrightarrow & \Resultat{x = 2,5}
\end{array}
\qq
\begin{array}[t]{crcl}
	& (x + 2)(3x - 1) & = & 3x^2 + 4x \\
	\Leftrightarrow & 3x^2 -x + 6x - 2  & = & 3x^2 + 4x \\
	\Leftrightarrow & 3x^2 + 5x -2 + 2 -3x^2 - 4x & = & 3x^2 - 3x^2 + 4x - 4x + 2  \\
	\Leftrightarrow & \Resultat{x = 2}
\end{array}
\]

%----
\dotfill\bigskip
%----

\begin{center}
	\textbf{\bsc{Sujet B}}
\end{center}

\textbf{Développements :}
\[
\begin{array}[t]{rcl}
	A(x) & = & 4(3x - 2) \\
	A(x) & = & 4 \times 3x - 4 \times 2 \\
	\Resultat{A(x) = 12x - 8}
\end{array}
\qq
\begin{array}[t]{rcl}
	B(x) & = & (2x + 6)(-4x - 1) \\
	B(x) & = & -8x^2 - 2x - 24x - 6 \\
	\Resultat{B(x) = -8x^2 - 26x - 6}
\end{array}
\qq
\begin{array}[t]{rcl}
	C(x) & = & (4 - 3x)^2 \\
	C(x) & = & 4^2 - 2 \times 4 \times 3x + (3x)^2\\
	\Resultat{C(x) = 9x^2 - 24x + 16}
\end{array}
\]

\textbf{Factorisations :}
\[
\begin{array}[t]{rcl}
	D(x) & = & 6x + 12 \\
	D(x) & = & 6x + 6 \times 2 \\
	\Resultat{D(x) = 6(x + 2)}
\end{array}
\qq
\begin{array}[t]{rcl}
	E(x) & = & (3x - 1)(2x - 4) + (3x - 1)(x + 3) \\
	E(x) & = & (3x - 1)[(2x - 4) + (x + 3)] \\
	E(x) & = & (3x - 1)(2x - 4 + x + 3) \\
	\Resultat{E(x) = (3x - 1)(3x - 1) = (3x - 1)^2}
\end{array}
\qq
\begin{array}[t]{rcl}
	F(x) & = & (2x - 4)^2 - (x + 3)^2 \\
	F(x) & = & [(2x - 4) + (x + 3)] \times [(2x - 4) - (x + 3)] \\
	F(x) & = & (2x - 4 + x + 3)(2x - 4 - x - 3) \\
	\Resultat{F(x) = (3x - 1)(x - 7)}
\end{array}
\]

\textbf{\'Equations :}
\[\begin{array}[t]{crcl}
	& 5x - 7 & = & 9 \\
	\Leftrightarrow & 5x - 7 + 7 & = & 9 + 7 \\
	\Leftrightarrow & 5x & = & 16 \\
	\Leftrightarrow & x & = & \frac{16}{5} \\
	\Leftrightarrow & \Resultat{x = 3,2}
\end{array}
\qq
\begin{array}[t]{crcl}
	& (2x + 1)(3x - 1) & = & 6x^2 + 4x \\
	\Leftrightarrow & 6x^2 -2x + 3x - 1  & = & 6x^2 + 4x \\
	\Leftrightarrow & 6x^2 + x - 1 + 1 -6x^2 - 4x & = & 6x^2 - 6x^2 + 4x - 4x + 1  \\
	\Leftrightarrow & -3x & = & 1 \\
	\Leftrightarrow & \Resultat{x = - \frac 1 3}
\end{array}
\]
\end{document} 