$\left\lVert \overrightarrow{AB} \right\rVert = AB = \sqrt{(x_B - x_A)^2 + (y_B - y_A)^2}$

\medskip

$\left\lVert \lambda \overrightarrow{AB}\right\rVert =
\left\lvert \lambda \right\rvert \times \left\lVert \overrightarrow{AB}\right\rVert$\par\medskip
Cela est évidemment valable dans un repère
$\left(O ; \overrightarrow\imath, \overrightarrow\jmath\right)$.\medskip

$\varnothing = \emptyset \subset \mathds N \subset \mathds Z \subset
\mathds D \subset \mathds Q\subset \mathds R \subset \mathds C$