$\overrightarrow{AB} + \overrightarrow{BC} = \overrightarrow{AC}$\medskip

$\overrightarrow{AB}\binom{x_B - x_A}{y_B - y_A}$ \quad donc \quad
$\overrightarrow{AB}\dbinom{x_B - x_A}{y_B - y_A}$\par\medskip
$\left\lVert \overrightarrow{AB} \right\rVert = AB = \sqrt{(x_B - x_A)^2 + (y_B - y_A)^2}$

\medskip

$\left\lVert \lambda \overrightarrow{AB}\right\rVert =
\left\lvert \lambda \right\rvert \times \left\lVert \overrightarrow{AB}\right\rVert$\par\medskip
Cela est évidemment valable dans un repère
$\left(O ; \overrightarrow\imath, \overrightarrow\jmath\right)$.\medskip

$\varnothing = \emptyset \subset \mathds N \subset \mathds Z \subset
\mathds D \subset \mathds Q\subset \mathds R \subset \mathds C$ \medskip

$\mathds R^*=]-\infty ; 0[ \cup ]0 ; +\infty[ = \mathds R \setminus \{0\}$.\medskip

$]-\infty ; 4] \cap ]-2 ; +\infty[ = ]-2 ; 4]$.\medskip

$\frac 1 2 \in \mathds Q$ mais $\frac 1 2 \notin \mathds Z$\medskip

$f\colon x \mapsto f(x)$ est définie sur $\mathcal D_f$.
On note $\mathcal C$ sa courbe représentative.