\'Equation de la tangente en $x_0$ :
$y = f'(x_0) \left(x - x_0\right) + f(x_0)$ avec
$f' = \left(\dfrac u v\right)' = \dfrac{u'v - uv'}{v^2}$.\medskip

$\Delta = b^2 - 4ac$. Si $\Delta > 0$ alors
$x = \dfrac{-b \pm \sqrt \Delta}{2a}$.\medskip

$\overrightarrow{AB} \cdot \overrightarrow{CD} = xx' + yy'$.\medskip

$u_{n + 1} = q\times u_n = u_0 \times q^{n+1}$.\medskip

$1 + q + q^2 + \dots + q^n = \sum_{i = 0}^n q^i$\medskip

$\mathds P(X = k) = \binom n k \times p^k \times (1-p)^{n-k}$.\medskip

$X$ suit la loi binomiale de param√®tres $n=10$ et $p=0,2$ :
$X \hookrightarrow \mathcal B(10 ; 0,2)$.