$\overrightarrow{AB} + \overrightarrow{BC} = \overrightarrow{AC}$\medskip

$\overrightarrow{AB}\binom{x_B - x_A}{y_B - y_A}$ \quad donc \quad
$\overrightarrow{AB}\dbinom{x_B - x_A}{y_B - y_A}$\par\medskip
$\left\lVert \overrightarrow{AB} \right\rVert = AB = \sqrt{(x_B - x_A)^2 + (y_B - y_A)^2}$

\medskip

$\left\lVert \lambda \overrightarrow{AB}\right\rVert =
\left\lvert \lambda \right\rvert \times \left\lVert \overrightarrow{AB}\right\rVert$\par\medskip
Cela est évidemment valable dans un repère orthonormé
$\left(O ; \overrightarrow\imath, \overrightarrow\jmath\right)$.